\begin{figure*}[t]
    \begin{tabular}{r c l}
    $\invUNFSymbol$(!var!$_{\Gamma,i}$) &=& $x_i$: !Ti! \\
    && if $x_i$: !Ti! is the $i$-th element of the context $\Gamma$ \\
    $\invUNFSymbol$(!op!$_{\Gamma,n}$) &=& !op!$_n(y_k,...,y_{k+n})$ \\
    && where $(y_k,...,y_{k+n})$ are the last $n$ variables of $\Gamma$ \\ 
    $\invUNFSymbol$(!e1;e2!) &=& !let x,Y = !$\invUNFSymbol$(!e1!) !in! $\invUNFSymbol$(!e2!) \\ 
    && TODO: \\ 
    $\invUNFSymbol$(!map!$_{\Gamma,x.e}$) &=& !map (x.e) X! \\ 
    $\invUNFSymbol$(!map2!$_{\Gamma,x,y.e}$) &=& !map2 (x,y.e) X1 X2! \\ 
    $\invUNFSymbol$(!foldl!$_{\Gamma,x,y.e}$) &=& !foldl (x,y.e) z X! \\ 
    $\invUNFSymbol$(!< e1, e2>!) &=& <$\invUNFSymbol$(!e1!), $\invUNFSymbol$(!e2!)> \\ 
    $\invUNFSymbol$(!J!$^T$!var!$_{\Gamma,i}$) &=& !fun Y -> fun (x1:T1,...,xm:Tm,z:Ti) ->!\\ 
    && !Y(x1,...,x(i-i),xi+z,x(i+1),...,xm)! \\
    $\invUNFSymbol$(!J!$^T$!op!$_{\Gamma,n}$) &=& !fun Y -> fun (x1:T1,...,xm:Tm,z:Ti) ->!\\ 
    && Y$(x_1,...,x_{m-n},x_{m-n+1}+\partial_1op_n*z,...,xm+\partial_nop_n*z)$ \\
    && where $\partial_iop_n$ is the $i$-th partial derivative of $op_n$ \\
    $\invUNFSymbol$(!J!$^T$!map!$_{\Gamma,x.e}$) &=&  !fun Y -> fun (x1:T1,...,xm:Tm,X',Z) ->!\\
    && Y((x1,...,xm)+$\nabla_{\Gamma}e *$(!reduce! + 0 Z),\\
    && !map2 (fun (a,b) -> a+!$\nabla_{\{x\}}e *$!b) X' Z'!) \\
    $\invUNFSymbol$(!J!$^T$!map2!$_{\Gamma,x,y.e}$) &=&  !fun Y -> fun (x1:T1,...,xm:Tm,X1',X2',Z) ->!\\
    && Y((x1,...,xm)+$\nabla_{\Gamma}e *$(!reduce! + 0 Z),\\
    && !map2 (fun (a,b) -> a+!$\nabla_{\{x1\}}e *$!b) X1' Z'!, \\
    && !map2 (fun (a,b) -> a+!$\nabla_{\{x2\}}e *$!b) X2' Z'!) \\
    && where $X1'$, $X2'$ are the tangent arrays for the two arrays arguments \\
    && of !map2! and $Z$ the tangent part for the return array of !map2! \\
    $\invUNFSymbol$(!J!$^T$!foldl!$_{\Gamma,x,y.e1}$) &=&  !fun Y -> fun (x1:T1,...,xm:Tm,X',z) ->!\\
    && !let A = scanl (fun (x,y) -> e1) e2 e3 in! \\
    && !let B = map2 (fun (x,y) ->! $\nabla_{\{x1\}}$!e1(x,y)) A e3 in!\\
    && !let C = shift1 (map2 (fun (x,y) ->! $\nabla_{\{x2\}}$!e1(x,y)) A e3) in!\\
    && !let D = scanr (fun (x,y) -> x*y) 1 B in!\\
    && Y(x1,...,xm, !map3 (fun (a,b,c) -> a+b*c*z) X' D C!)
    \end{tabular}
    \caption{UNF transformation from Target UNF to Target}
    \label{fig:unf_to_target}
    \end{figure*}